src/tls/HSL.Receive.fsti
@@ -22,7 +22,13 @@ module HSM13 = Parsers.Handshake13
 
 /// HSL main API
 
-type lbuffer8 (l:uint_32) = b:B.buffer uint_8{B.len b == l}
+type slice =
+  sl:LP.slice
+       (LP.srel_of_buffer_srel (B.trivial_preorder LP.byte))
+       (LP.srel_of_buffer_srel (B.trivial_preorder LP.byte)){
+         v sl.LP.len <= v LP.validator_max_length
+     }
+
 
 /// For incremental parsing, flight receiving functions have
 ///   preconditions on the current in-progress flight
@@ -51,7 +57,6 @@ val parsed_bytes (st:hsl_state) (h:HS.mem) : GTot bytes
 
 let length_parsed_bytes (st:hsl_state) (h:HS.mem) : GTot nat =
   Seq.length (parsed_bytes st h)
-
 
 val in_progress_flt (st:hsl_state) (h:HS.mem) : GTot in_progress_flt_t
 
@@ -108,48 +113,54 @@ val create (r:Mem.rgn)
 
 /// Receive API
 
-type b8 = B.buffer uint_8
-
 #push-options "--max_ifuel 2 --initial_ifuel 2 --z3rlimit 20"  //increase ifuel for inverting options and tuples
 
 unfold
-let basic_pre_post (st:hsl_state) (b:b8) (from to:uint_32) : HS.mem -> Type0
+let basic_pre_post (st:hsl_state) (b:slice) (from to:uint_32) (in_progress:in_progress_flt_t)
+  : HS.mem -> Type0
   = fun h ->
-    let open B in
+    let open B in let open LP in
+    
     invariant st h /\
-    loc_disjoint (footprint st) (loc_buffer b) /\
+
+    live_slice h b /\
+    loc_disjoint (footprint st) (loc_buffer b.base) /\
+    
     v from + length_parsed_bytes st h <= v to /\
-    to <= len b /\
-    Seq.equal (Seq.slice (as_seq h b)
+    v to <= v b.len /\
+    
+    Seq.equal (Seq.slice (as_seq h b.base)
                          (v from)
                          (v from + length_parsed_bytes st h))
-              (parsed_bytes st h)
+              (parsed_bytes st h) /\
+
+    (in_progress_flt st h == F_none \/ in_progress_flt st h == in_progress)
+
 
 let valid_flight_t 'a =
-  (flt:'a) -> (from:uint_32) -> (to:uint_32) -> (b:b8) -> (h:HS.mem) -> Type0
+  (flt:'a) -> (from:uint_32) -> (to:uint_32) -> (b:slice) -> (h:HS.mem) -> Type0
 
 unfold private
 let receive_post 
   (st:hsl_state)
-  (b:b8)
+  (b:slice)
   (from to:uint_32)
   (f:valid_flight_t 'a)
   (in_progress:in_progress_flt_t)
   (h0:HS.mem)
   (x:TLSError.result (option 'a))
   (h1:HS.mem)
-  = basic_pre_post st b from to h0 /\
-    B.modifies (footprint st) h0 h1 /\  //only local footprint is modified
+  = basic_pre_post st b from to in_progress h0 /\
+    B.modifies (footprint st) h0 h1 /\
     (let open FStar.Error in
      match x with
-     | Error _ -> True  //underspecified
-     | Correct None ->  //waiting for more data
+     | Error _ -> True
+     | Correct None ->
        in_progress_flt st h1 == in_progress /\
        parsed_bytes st h1 ==
-         Seq.slice (B.as_seq h0 b) (v from) (v to)
+         Seq.slice (B.as_seq h0 b.LP.base) (v from) (v to)
      | Correct (Some flt) ->
-       f flt from to b h1 /\  //flight specific postcondition
-       //Internal state for partial parse is reset, ready to receive another flight
+       f flt from to b h1 /\
        parsed_bytes st h1 == Seq.empty /\
        in_progress_flt st h1 == F_none
      | _ -> False)
@@ -161,19 +172,18 @@ let receive_post
 
 /// First 13 flights
 
-/// Common function for buffer being a valid 13 message msg
+/// Common function for slice being a valid 13 message msg
 
 let valid_parsing13
   (msg:HSM13.handshake13)
-  (buf:b8)
+  (buf:slice)
   (from to:uint_32)
   (h:HS.mem)
   = let parser = HSM13.handshake13_parser in
-    let slice = LP.make_slice buf (B.len buf) in
     from <= to /\
-    LP.valid parser h slice from /\
-    LP.contents parser h slice from == msg /\
-    LP.content_length parser h slice from == UInt32.v (to - from)
+    LP.valid parser h buf from /\
+    LP.contents parser h buf from == msg /\
+    LP.content_length parser h buf from == UInt32.v (to - from)
 
 
 (****** Flight [ EncryptedExtensions; Certificate13; CertificateVerify; Finished ] ******)
@@ -198,7 +208,7 @@ type flight13_ee_c_cv_fin = {
 
 let valid_flight13_ee_c_cv_fin
   : valid_flight_t flight13_ee_c_cv_fin
-  = fun (flt:flight13_ee_c_cv_fin) (from to:uint_32) (b:b8) (h:HS.mem) ->
+  = fun (flt:flight13_ee_c_cv_fin) (from to:uint_32) (b:slice) (h:HS.mem) ->
 
     valid_parsing13 (HSM13.M_encrypted_extensions (G.reveal flt.ee_msg)) b from flt.begin_c h /\
     valid_parsing13 (HSM13.M_certificate (G.reveal flt.c_msg)) b flt.begin_c flt.begin_cv h /\
@@ -207,9 +217,9 @@ let valid_flight13_ee_c_cv_fin
 
 
 val receive_flight13_ee_c_cv_fin
-  (st:hsl_state) (b:b8) (from to:uint_32)
+  (st:hsl_state) (b:slice) (from to:uint_32)
   : ST (TLSError.result (option flight13_ee_c_cv_fin))
-       (requires basic_pre_post st b from to)
+       (requires basic_pre_post st b from to F13_ee_c_cv_fin)
        (ensures  receive_post st b from to valid_flight13_ee_c_cv_fin F13_ee_c_cv_fin)
 
 
@@ -234,7 +244,7 @@ type flight13_ee_cr_c_cv_fin = {
 
 let valid_flight13_ee_cr_c_cv_fin
   : valid_flight_t flight13_ee_cr_c_cv_fin
-  = fun (flt:flight13_ee_cr_c_cv_fin) (from to:uint_32) (b:b8) (h:HS.mem) ->
+  = fun (flt:flight13_ee_cr_c_cv_fin) (from to:uint_32) (b:slice) (h:HS.mem) ->
 
     valid_parsing13 (HSM13.M_encrypted_extensions (G.reveal flt.ee_msg)) b from flt.begin_cr h /\
     valid_parsing13 (HSM13.M_certificate_request (G.reveal flt.cr_msg)) b flt.begin_cr flt.begin_c h /\
@@ -244,9 +254,9 @@ let valid_flight13_ee_cr_c_cv_fin
 
 
 val receive_flight13_ee_cr_c_cv_fin
-  (st:hsl_state) (b:b8) (from to:uint_32)
+  (st:hsl_state) (b:slice) (from to:uint_32)
   : ST (TLSError.result (option flight13_ee_cr_c_cv_fin))
-       (requires basic_pre_post st b from to)
+       (requires basic_pre_post st b from to F13_ee_cr_c_cv_fin)
        (ensures  receive_post st b from to valid_flight13_ee_cr_c_cv_fin F13_ee_cr_c_cv_fin)
 
 
@@ -261,14 +271,14 @@ type flight13_ee_fin = {
 }
 
 let valid_flight13_ee_fin : valid_flight_t flight13_ee_fin =
-  fun (flt:flight13_ee_fin) (from to:uint_32) (b:b8) (h:HS.mem) ->
+  fun (flt:flight13_ee_fin) (from to:uint_32) (b:slice) (h:HS.mem) ->
 
   valid_parsing13 (HSM13.M_encrypted_extensions (G.reveal flt.ee_msg)) b from flt.begin_fin h /\
   valid_parsing13 (HSM13.M_finished (G.reveal flt.fin_msg)) b flt.begin_fin to h
 
-val receive_flight13_ee_fin (st:hsl_state) (b:b8) (from to:uint_32)
+val receive_flight13_ee_fin (st:hsl_state) (b:slice) (from to:uint_32)
   : ST (TLSError.result (option flight13_ee_fin))
-       (requires basic_pre_post st b  from to)
+       (requires basic_pre_post st b from to F13_ee_fin)
        (ensures  receive_post st b from to valid_flight13_ee_fin F13_ee_fin)
 
 
@@ -281,13 +291,13 @@ type flight13_fin = {
 
 
 let valid_flight13_fin : valid_flight_t flight13_fin =
-  fun (flt:flight13_fin) (from to:uint_32) (b:b8) (h:HS.mem) ->
+  fun (flt:flight13_fin) (from to:uint_32) (b:slice) (h:HS.mem) ->
 
   valid_parsing13 (HSM13.M_finished (G.reveal flt.fin_msg)) b from to h
 
-val receive_flight13_fin (st:hsl_state) (b:b8) (from to:uint_32)
+val receive_flight13_fin (st:hsl_state) (b:slice) (from to:uint_32)
   : ST (TLSError.result (option flight13_fin))
-       (requires basic_pre_post st b  from to)
+       (requires basic_pre_post st b from to F13_fin)
        (ensures  receive_post st b from to valid_flight13_fin F13_fin)
 
 
@@ -306,7 +316,7 @@ type flight13_c_cv_fin = {
 
 let valid_flight13_c_cv_fin
   : valid_flight_t flight13_c_cv_fin
-  = fun (flt:flight13_c_cv_fin) (from to:uint_32) (b:b8) (h:HS.mem) ->
+  = fun (flt:flight13_c_cv_fin) (from to:uint_32) (b:slice) (h:HS.mem) ->
 
     valid_parsing13 (HSM13.M_certificate (G.reveal flt.c_msg)) b from flt.begin_cv h /\
     valid_parsing13 (HSM13.M_certificate_verify (G.reveal flt.cv_msg)) b flt.begin_cv flt.begin_fin h /\
@@ -314,9 +324,9 @@ let valid_flight13_c_cv_fin
 
 
 val receive_flight13_c_cv_fin
-  (st:hsl_state) (b:b8) (from to:uint_32)
+  (st:hsl_state) (b:slice) (from to:uint_32)
   : ST (TLSError.result (option flight13_c_cv_fin))
-       (requires basic_pre_post st b from to)
+       (requires basic_pre_post st b from to F13_c_cv_fin)
        (ensures  receive_post st b from to valid_flight13_c_cv_fin F13_c_cv_fin)
 
 
@@ -331,13 +341,13 @@ type flight13_eoed = {
 
 
 let valid_flight13_eoed : valid_flight_t flight13_eoed =
-  fun (flt:flight13_eoed) (from to:uint_32) (b:b8) (h:HS.mem) ->
+  fun (flt:flight13_eoed) (from to:uint_32) (b:slice) (h:HS.mem) ->
 
   valid_parsing13 (HSM13.M_end_of_early_data (G.reveal flt.eoed_msg)) b from to h
 
-val receive_flight13_eoed (st:hsl_state) (b:b8) (from to:uint_32)
+val receive_flight13_eoed (st:hsl_state) (b:slice) (from to:uint_32)
   : ST (TLSError.result (option flight13_eoed))
-       (requires basic_pre_post st b  from to)
+       (requires basic_pre_post st b from to F13_eoed)
        (ensures  receive_post st b from to valid_flight13_eoed F13_eoed)
 
 
@@ -352,13 +362,13 @@ type flight13_nst = {
 
 
 let valid_flight13_nst : valid_flight_t flight13_nst =
-  fun (flt:flight13_nst) (from to:uint_32) (b:b8) (h:HS.mem) ->
+  fun (flt:flight13_nst) (from to:uint_32) (b:slice) (h:HS.mem) ->
 
   valid_parsing13 (HSM13.M_new_session_ticket (G.reveal flt.nst_msg)) b from to h
 
-val receive_flight13_nst (st:hsl_state) (b:b8) (from to:uint_32)
+val receive_flight13_nst (st:hsl_state) (b:slice) (from to:uint_32)
   : ST (TLSError.result (option flight13_nst))
-       (requires basic_pre_post st b  from to)
+       (requires basic_pre_post st b from to F13_nst)
        (ensures  receive_post st b from to valid_flight13_nst F13_nst)
 
 
